src/Narcissus/Examples/NetworkStack/IPv4Header.v
@@ -90,337 +90,6 @@ Definition IPv4_encoder_impl {sz} v r :=
   Eval simpl in (projT1 IPv4_encoder sz v 0 r tt).
 Print IPv4_encoder_impl.
 
-(*Lemma sequence_Compose_format_refined_decode_correct
-      {cache : Cache}
-      {S V1 V2 T : Type}
-      {P : CacheDecode -> Prop}
-      {P_inv1 P_inv2 : (CacheDecode -> Prop) -> Prop}
-      (P_inv_pf : cache_inv_Property P (fun P => P_inv1 P /\ P_inv2 P))
-      (monoid : Monoid T)
-      (view1 : S -> V1)
-      (view2 : S -> V2 -> Prop)
-      (Source_Predicate : S -> Prop)
-      (View_Predicate1 : V1 -> Prop)
-      (View_Predicate2 : V2 -> Prop)
-      (format1 : FormatM V1 T)
-      (format2 : FormatM S T )
-      (subformat : FormatM S T )
-      (decode1 : DecodeM (V1 * T) T)
-      (decode_1_OK :
-         cache_inv_Property P P_inv1
-         -> CorrectDecoder monoid View_Predicate1 View_Predicate1 eq format1 decode1 P format1)
-      (View_Predicate1_OK : forall (s : S), Source_Predicate s -> View_Predicate1 (view1 s))
-
-      (view_format : FormatM V2 T)
-      (decode2 : DecodeM (V2 * T) T)
-      (decode_2_OK :
-           cache_inv_Property P P_inv2 ->
-         CorrectRefinedDecoder monoid Source_Predicate
-                               View_Predicate2
-                               view2 format2 subformat decode2 P view_format)
-  : CorrectRefinedDecoder
-      monoid
-      Source_Predicate
-      View_Predicate2
-      view2
-      (Projection_Format format1 view1 ++ format2)%format
-      (Projection_Format format1 view1 ++ subformat)%format
-      (Compose_Decode (sequence_Decode' decode1 (fun _ => decode2))
-                      (fun vt => ((snd (fst vt), snd vt))))
-      P (Compose_Format format1 (fun _ _ => True) ++ view_format)%format.
-Proof.
-  specialize (decode_1_OK (proj1 P_inv_pf)).
-  specialize (decode_2_OK (proj2 P_inv_pf)).
-  destruct decode_2_OK as [decode_2_OK ?].
-  split.
-  - eapply injection_decode_correct.
-    + eapply Sequence_decode_correct.
-      * eassumption.
-      * intros; eapply Compose_decode_correct; eauto.
-        intros; subst; eauto.
-      * simpl; intros; instantiate (1 := fun v1 s => view1 s = v1);
-          simpl; eauto.
-      * intros. simpl.
-        instantiate (3 := fun _ => View_Predicate2).
-        instantiate (2 := fun _ => view2).
-        instantiate (1 := fun _ => view_format).
-        eapply weaken_source_pred; eauto.
-        unfold flip, impl, pointwise_relation; intuition.
-      * intros.
-        instantiate (1 := (Projection_Format format1 fst ++ Projection_Format view_format snd)%format).
-        unfold sequence_Format, ComposeOpt.compose, Bind2;
-          apply unfold_computes; computes_to_econstructor.
-        unfold Projection_Format, Compose_Format; apply unfold_computes.
-        eexists _; simpl; intuition eauto.
-        apply unfold_computes; eauto.
-        computes_to_econstructor.
-        unfold Projection_Format, Compose_Format; apply unfold_computes.
-        eexists _; simpl; intuition eauto.
-        apply unfold_computes; eauto.
-        reflexivity.
-    + simpl; intros; intuition.
-    + simpl; intros; intuition.
-    + simpl; intros.
-      unfold sequence_Format, ComposeOpt.compose, Bind2,
-      Projection_Format, Compose_Format in *; computes_to_inv.
-      rewrite -> unfold_computes in H0'; destruct_ex; split_and;
-        subst.
-      rewrite -> unfold_computes in H0; destruct_ex; split_and;
-        subst.
-      destruct v1; destruct v0; simpl in *; computes_to_econstructor.
-      apply unfold_computes.
-      eexists; eauto.
-      computes_to_econstructor; eauto.
-  - intros.
-    unfold sequence_Format, ComposeOpt.compose, Bind2,
-      Projection_Format, Compose_Format in *; computes_to_inv.
-    rewrite -> unfold_computes in H0; destruct_ex; split_and;
-      subst; injections; destruct v0; destruct v; simpl in *.
-    eapply H in H0'; destruct_ex; split_and; subst.
-    setoid_rewrite mappend_assoc.
-    eexists _, _, _; split; eauto.
-    computes_to_econstructor.
-    apply unfold_computes; eexists; eauto.
-    computes_to_econstructor; eauto.
-Qed.
-
-Lemma sequence_Compose_format_decode_correct''
-      {cache : Cache}
-      {S V1 V2 T : Type}
-      {P : CacheDecode -> Prop}
-      {P_inv1 P_inv2 : (CacheDecode -> Prop) -> Prop}
-      (P_inv_pf : cache_inv_Property P (fun P => P_inv1 P /\ P_inv2 P))
-      (monoid : Monoid T)
-      (view1 : S -> V1)
-      (view : S -> V2 -> Prop)
-      (Source_Predicate : S -> Prop)
-      (View_Predicate1  : V1 -> Prop)
-      (View_Predicate2  : V2 -> Prop)
-      (format1 : FormatM V1 T)
-      (format2 : FormatM S T )
-      (decode1 : DecodeM (V1 * T) T)
-      (view_format : FormatM V2 T)
-      (decode_1_OK :
-         cache_inv_Property P P_inv1
-         -> CorrectDecoder monoid View_Predicate1 View_Predicate1 eq format1 decode1 P format1)
-      (View_Predicate_OK : forall s v, Source_Predicate s ->
-                                       IsProj view1 v s  ->
-                                       View_Predicate1 v)
-      (decode2 : V1 -> DecodeM (V2 * T) T)
-      (decode2_pf : forall v1 : V1,
-          cache_inv_Property P P_inv2 ->
-          View_Predicate1 v1 ->
-          CorrectDecoder monoid (fun s => Source_Predicate s
-                                          /\ IsProj view1 v1 s)
-                         View_Predicate2
-                         view format2 (decode2 v1) P view_format)
-  : CorrectDecoder
-      monoid
-      Source_Predicate
-      View_Predicate2
-      view
-      (Projection_Format format1 view1 ++ format2)%format
-      (sequence_Decode decode1 decode2)
-      P (Compose_Format format1 (fun _ _ => True) ++ view_format)%format.
-Proof.
-  Opaque CorrectDecoder.
-  eapply Sequence_decode_correct. with (view1 := view)
-                                      (view2 := fun _ => eq)
-                                      (View_Predicate2 := fun v1 v2 => Source_Predicate v2 /\
-                                                                       view v2 v1)
-                                      (consistency_predicate := fun v1 s => view s v1);
-    try eassumption; eauto.
-  - intros; eapply Compose_decode_correct; try eassumption;
-    intros; eauto.
-  - instantiate (1 := fun _ => format2); eauto.
-  - simpl; intros.
-    unfold sequence_Format, ComposeOpt.compose, Bind2,
-    Projection_Format, Compose_Format.
-    apply unfold_computes.
-    apply unfold_computes in H.
-    apply unfold_computes in H0.
-    eauto.
-Qed.
-
-Lemma sequence_Compose_format_refined_decode_correct_finish
-      {cache : Cache}
-      {S V1 T : Type}
-      {P : CacheDecode -> Prop}
-      {P_inv1 P_inv2 : (CacheDecode -> Prop) -> Prop}
-      (P_inv_pf : cache_inv_Property P (fun P => P_inv1 P /\ P_inv2 P))
-      (monoid : Monoid T)
-      (view1 : S -> V1)
-      (view : S -> V1 -> Prop)
-      (Source_Predicate : S -> Prop)
-      (View_Predicate1 : V1 -> Prop)
-      (View_Predicate' : V1 -> Prop)
-      (format1 : FormatM V1 T)
-      (format2 : FormatM S T )
-      (decode1 : DecodeM (V1 * T) T)
-      (view_format : FormatM V1 T)
-      (decode_1_OK :
-         cache_inv_Property P P_inv1
-         -> CorrectDecoder monoid View_Predicate1 View_Predicate1 eq format1 decode1 P format1)
-      (view_OK : forall v s, IsProj view1 s v -> view v s)
-      (View_Predicate1_OK : forall (s : S), Source_Predicate s -> View_Predicate1 (view1 s))
-      (*view_format_OK : forall v t env,
-          format1 v env t ->
-          View_Predicate' v ->
-          view_format v env t*)
-      (View_Predicate'_OK :
-         forall s v, Source_Predicate s -> view s v -> View_Predicate' v)
-      (View_Predicate'_OK_2 :
-         forall v, View_Predicate1 v -> View_Predicate' v)
-  : CorrectRefinedDecoder
-      monoid
-      Source_Predicate
-      View_Predicate'
-      view
-      (Projection_Format format1 view1 ++ format2)%format
-      (Projection_Format format1 view1)%format
-      decode1
-      P view_format%format.
-Proof.
-  specialize (decode_1_OK (proj1 P_inv_pf)).
-  split.
-  - eapply weaken_view_pred.
-    unfold pointwise_relation, impl; intros.
-    eauto.
-    eapply format_decode_correct_alt'.
-    7: { eapply projection_decode_correct.
-         eapply decode_1_OK.
-         intros.
-         eapply View_Predicate1_OK.
-         apply H. }
-    all: unfold flip, pointwise_relation, impl; intuition eauto.
-    unfold Projection_Format; eapply EquivFormat_reflexive.
-    unfold Projection_Format; eapply EquivFormat_reflexive.
-  - intros.
-    unfold sequence_Format, ComposeOpt.compose, Bind2,
-      Projection_Format, Compose_Format in *; computes_to_inv.
-    rewrite -> unfold_computes in H; destruct_ex; split_and;
-      subst; injections; destruct v0; destruct v; simpl in *.
-    eexists _, _, _; split; eauto.
-    apply unfold_computes.
-    eexists _; intuition eauto.
-Qed.
-
-Lemma IPv4_Packet_measure_decode_OK
-  : forall P,
-    {decode : _ & {subformat : _ &
-                 {P_inv : _ &
-                          { view_format : _ &
-                 cache_inv_Property P P_inv ->
-                 CorrectRefinedDecoder monoid IPv4_Packet_OK (constant True) (constant (constant True))
-    ((format_nat 4 ◦ constant 4 ++
-                 format_nat 4 ◦ Init.Nat.add 5 ◦ Datatypes.length (A:=word 32) ◦ Options ++
-      format_unused_word 8 ++
-      format_word ◦ TotalLength ++
-      format_word ◦ ID ++
-      format_unused_word 1 ++
-      format_bool ◦ DF ++
-      format_bool ◦ MF ++ format_word ◦ FragmentOffset ++ format_word ◦ TTL ++ format_enum ProtocolTypeCodes ◦ Protocol) ++
-                                                                                                                         format_unused_word 16 ++ format_word ◦ SourceAddress ++ format_word ◦ DestAddress ++ format_list format_word ◦ Options)%format
-    subformat
-    (*(format_word ◦ constant natToWord 4 4
-                      ++
-                      ((format_nat 4 ◦ Init.Nat.add 5) ◦ Datatypes.length (A:=word 32)) ◦ Options)%format *)
-    decode
-    (*fun t env =>
-       `(_, t', env') <- decode_nat 4 t env;
-         `(n, _, _) <- decode_nat 4 t' env';
-         Some (n * 32, t, env)*) P
-    view_format /\
-                 (forall n env t,
-                     view_format n env t ->
-                     forall (a : IPv4_Packet) (t1 t2 : ByteString * CacheFormat),
-               word 16 ->
-               IPv4_Packet_OK a ->
-               (format_nat 4 ◦ constant 4 ++
-                format_nat 4 ◦ Init.Nat.add 5 ◦ Datatypes.length (A:=word 32) ◦ Options ++
-                format_unused_word 8 ++
-                format_word ◦ TotalLength ++
-                format_word ◦ ID ++
-                format_unused_word 1 ++
-                format_bool ◦ DF ++
-                format_bool ◦ MF ++ format_word ◦ FragmentOffset ++ format_word ◦ TTL ++ format_enum ProtocolTypeCodes ◦ Protocol)%format
-                 a env t1 ->
-               (format_word ◦ SourceAddress ++ format_word ◦ DestAddress ++ format_list format_word ◦ Options)%format a
-                 (addE (snd t1) 16) t2 ->
-               (constant (4 + (4 + (8 + (16 + (16 + (1 + (1 + (1 + (13 + (8 + 8))))))))))) a + 16 +
-               (fun a0 : IPv4_Packet => 32 + (32 + (| Options a0 |) * 32)) a = n * 8)}}}}.
-Proof.
-  intros; eexists _, _, _, _; intros.
-  split.
-  match goal with
-         | |- CorrectRefinedDecoder ?monoid _ _ _ _ _ _ _ _ =>
-           intros; eapply format_decode_refined_correct_refineEquiv; unfold flip;
-             repeat (normalize_step monoid)
-         end.
-  eapply (sequence_Compose_format_refined_decode_correct H);
-    [ intros; apply_rules
-      | solve_data_inv
-      | intros ].
-  match goal with
-  | |- CorrectRefinedDecoder ?monoid _ _ _ _ _ _ _ _ =>
-    intros; eapply format_decode_refined_correct_refineEquiv; unfold flip
-  end.
-  eapply EquivFormat_UnderSequence'.
-  eapply EquivFormat_trans.
-  eapply EquivFormat_compose_map.
-  apply EquivFormat_reflexive.
-  apply EquivFormat_reflexive.
-  eapply (sequence_Compose_format_refined_decode_correct_finish H0).
-  intros. apply_rules.
-  solve_data_inv.
-  solve_data_inv.
-  intros; eapply H1.
-  solve_data_inv.
-  solve_data_inv.
-  admit.
-  intros.
-  unfold sequence_Format at 1 2, ComposeOpt.compose, Bind2 in H3;
-    apply unfold_computes in H3; computes_to_inv; subst.
-
-
-
-  [ intros; apply_rules
-    | try solve_data_inv
-      | intros ].
-  instantiate (1 := fun n env t =>
-
-                     forall (a : IPv4_Packet) (t1 t2 : ByteString * CacheFormat),
-               word 16 ->
-               IPv4_Packet_OK a ->
-               (format_nat 4 ◦ constant 4 ++
-                format_nat 4 ◦ Init.Nat.add 5 ◦ Datatypes.length (A:=word 32) ◦ Options ++
-                format_unused_word 8 ++
-                format_word ◦ TotalLength ++
-                format_word ◦ ID ++
-                format_unused_word 1 ++
-                format_bool ◦ DF ++
-                format_bool ◦ MF ++ format_word ◦ FragmentOffset ++ format_word ◦ TTL ++ format_enum ProtocolTypeCodes ◦ Protocol)%format
-                 a env t1 ->
-               (format_word ◦ SourceAddress ++ format_word ◦ DestAddress ++ format_list format_word ◦ Options)%format a
-                 (addE (snd t1) 16) t2 ->
-               (constant (4 + (4 + (8 + (16 + (16 + (1 + (1 + (1 + (13 + (8 + 8))))))))))) a + 16 +
-               (fun a0 : IPv4_Packet => 32 + (32 + (| Options a0 |) * 32)) a = n * 8).
-  eapply ExtractViewFromRefined; eauto.
-  intros.
-  apply unfold_computes; intros.
-
-
-
-  2: {
-       eapply (sequence_Compose_format_refined_decode_correct H).
-
-
-    (format_nat 4 ◦ constant 4
-               ++
-               ((format_nat 4 ◦ Init.Nat.add 5) ◦ Datatypes.length (A:=word 32)) ◦ Options)%format.
-  admit.
-Defined. *)
-
 Arguments andb : simpl never.
 
 (*Hint Extern 4 => eapply aligned_IPv4_Packet_encoded_measure_OK_1.
@@ -436,15 +105,41 @@ Ltac apply_new_combinator_rule ::=
     | repeat calculate_length_ByteString
     | solve_mod_8
     | solve_mod_8
-    |
+    | split
     | intros; NormalizeFormats.normalize_format; apply_rules ]
   end.
+
 
 (* Step Three: Synthesize a decoder and a proof that /it/ is correct. *)
 Definition IPv4_Packet_Header_decoder
   : CorrectAlignedDecoderFor IPv4_Packet_OK IPv4_Packet_Format.
 Proof.
   synthesize_aligned_decoder.
+  { intros.
+    match goal with
+    | |- CorrectRefinedDecoder ?monoid _ _ _ _ _ _ _ _ =>
+      intros; eapply format_decode_refined_correct_refineEquiv; unfold flip;
+        repeat (normalize_step monoid)
+    end.
+    eapply format_sequence_refined_correct.
+    apply H0.
+    intros; apply_rules.
+    solve_data_inv.
+    intros.
+    eapply format_sequence_refined_correct.
+    apply H1.
+    intros; apply_rules.
+    solve_data_inv.
+    intros; eapply ExtractViewFromRefined with (View_Predicate := fun _ => True); eauto.
+    intros; intuition.
+    instantiate (1 := v0 * 4).
+    unfold Basics.compose, IsProj in *.
+    unfold IPv4_Packet_OK in *.
+    omega. }
+  admit.
+  synthesize_cache_invariant.
+  cbv beta; unfold decode_nat, sequence_Decode; optimize_decoder_impl.
+  align_decoders.
 Defined.
 
 Print Assumptions IPv4_Packet_Header_decoder.
